change linear order instantiation of full total states to allow states in the trace to differ as long as they are ordered correctly, remove sorry for postcondition monotonicity
This change does not affect the addition of states. Thus, the order obtained via the addition is now different than the linear order in the case when the traces are not the same.
The change was needed to express a more general version of the inhale downward monotonicity.

TotalViperState.thy
@@ -122,13 +122,18 @@ begin
 definition less_eq_full_total_state_ext :: "('a,'b) full_total_state_ext \<Rightarrow> ('a,'b) full_total_state_ext \<Rightarrow> bool"
   where "\<omega>1 \<le> \<omega>2 \<equiv> 
          get_store_total \<omega>1 = get_store_total \<omega>2 \<and>
-         get_trace_total \<omega>1 = get_trace_total \<omega>2 \<and>
+         dom (get_trace_total \<omega>1) = dom (get_trace_total \<omega>2) \<and>
+         (\<forall>lbl \<phi> \<phi>'. (get_trace_total \<omega>1 lbl = Some \<phi> \<and> 
+                      get_trace_total \<omega>2 lbl = Some \<phi>') \<longrightarrow> \<phi> \<le> \<phi>') \<and>
          get_total_full \<omega>1 \<le> get_total_full \<omega>2 \<and>
          full_total_state.more \<omega>1 = full_total_state.more \<omega>2"
 
 definition less_full_total_state_ext :: "('a,'b) full_total_state_ext \<Rightarrow> ('a,'b) full_total_state_ext \<Rightarrow> bool"
   where "\<omega>1 < \<omega>2 \<equiv> 
-           \<omega>1 \<le> \<omega>2 \<and> get_total_full \<omega>1 < get_total_full \<omega>2 "
+           \<omega>1 \<le> \<omega>2 \<and> 
+           (get_total_full \<omega>1 < get_total_full \<omega>2 \<or>
+           (\<exists>lbl \<phi> \<phi>'. get_trace_total \<omega>1 lbl = Some \<phi> \<and> get_trace_total \<omega>2 lbl = Some \<phi>' \<and>
+                        \<phi> < \<phi>'))"
 
 instance
 proof
@@ -144,16 +149,19 @@ proof
         unfolding less_full_total_state_ext_def
         by simp
     next
-      from \<open>x < y\<close>
-      show "\<not> y \<le> x"
-        unfolding less_full_total_state_ext_def less_eq_full_total_state_ext_def
-        by fastforce
+      from \<open>x < y\<close> consider "get_total_full x < get_total_full y" |
+                            "(\<exists>lbl \<phi> \<phi>'. get_trace_total x lbl = Some \<phi> \<and> get_trace_total y lbl = Some \<phi>' \<and>
+                                         \<phi> < \<phi>')"
+        unfolding less_full_total_state_ext_def
+        by blast
+      thus "\<not> y \<le> x"
+        by (metis TotalViperState.less_eq_full_total_state_ext_def leD)
     qed
   next
     assume "x \<le> y \<and> \<not> y \<le> x"
     thus "x < y"
-    unfolding less_full_total_state_ext_def less_eq_full_total_state_ext_def    
-    by force
+      unfolding less_full_total_state_ext_def less_eq_full_total_state_ext_def
+      by fastforce
   qed
 
   show "x \<le> x"
@@ -161,17 +169,51 @@ proof
     by auto
 
   show "x \<le> y \<Longrightarrow> y \<le> z \<Longrightarrow> x \<le> z"
-    unfolding less_eq_full_total_state_ext_def
-    by (metis (mono_tags, opaque_lifting) dual_order.trans)
+  proof -
+    assume Leqs: "x \<le> y" "y \<le> z"
+
+    show "x \<le> z"
+      unfolding less_eq_full_total_state_ext_def
+    proof (intro conjI)
+      show "\<forall>lbl \<phi> \<phi>'. get_trace_total x lbl = Some \<phi> \<and> get_trace_total z lbl = Some \<phi>' \<longrightarrow> \<phi> \<le> \<phi>'"
+        using Leqs
+        unfolding less_eq_full_total_state_ext_def
+        by (metis (mono_tags, opaque_lifting) domIff dual_order.trans not_None_eq)
+    qed (insert Leqs[simplified less_eq_full_total_state_ext_def], auto)
+  qed
 
   show "x \<le> y \<Longrightarrow> y \<le> x \<Longrightarrow> x = y"
-    unfolding less_eq_full_total_state_ext_def
-    apply (rule full_total_state.equality)
-       apply blast
-      apply blast
-     apply fastforce
-    by blast
+  proof -
+    assume "x \<le> y" and "y \<le> x"
+
+    show ?thesis
+    proof (rule full_total_state.equality)
+      show "get_store_total x = get_store_total y"
+        using \<open>x \<le> y\<close> less_eq_full_total_state_ext_def by blast
+    
+      show "get_trace_total x = get_trace_total y"
+      proof -
+        have *: "\<And> lbl \<phi> \<phi>'. get_trace_total x lbl = Some \<phi> \<Longrightarrow> get_trace_total y lbl = Some \<phi>' \<Longrightarrow> \<phi> = \<phi>'"
+          using \<open>x \<le> y\<close> \<open>y \<le> x\<close> less_eq_full_total_state_ext_def
+          by fastforce
+        have DomEq: "dom (get_trace_total x) = dom (get_trace_total y)"
+          using \<open>x \<le> y\<close> less_eq_full_total_state_ext_def by blast
+        show ?thesis
+          apply (rule HOL.ext)
+          using * DomEq
+          by (metis domIff not_None_eq)
+      qed
+
+      show "get_total_full x = get_total_full y"
+        using \<open>x \<le> y\<close> \<open>y \<le> x\<close> less_eq_full_total_state_ext_def
+        by auto
+
+      show "full_total_state.more x = full_total_state.more y "
+        using \<open>x \<le> y\<close> less_eq_full_total_state_ext_def by blast
+    qed
+  qed         
 qed
+
 end
 
 lemma less_eq_total_stateI:
@@ -210,22 +252,37 @@ lemma less_eq_full_total_stateI:
      full_total_state.more \<omega>1 = full_total_state.more \<omega>2 \<Longrightarrow>
      \<omega>1 \<le> \<omega>2"
   unfolding less_eq_full_total_state_ext_def
-  by blast
+  by auto
+
+lemma less_eq_full_total_stateI2:
+    "get_store_total \<omega>1 = get_store_total \<omega>2 \<Longrightarrow>
+     dom (get_trace_total \<omega>1) = dom (get_trace_total \<omega>2) \<Longrightarrow>
+     (\<forall>lbl \<phi> \<phi>'. (get_trace_total \<omega>1 lbl = Some \<phi> \<and> 
+                      get_trace_total \<omega>2 lbl = Some \<phi>') \<longrightarrow> \<phi> \<le> \<phi>') \<Longrightarrow>
+     get_total_full \<omega>1 \<le> get_total_full \<omega>2 \<Longrightarrow>
+     full_total_state.more \<omega>1 = full_total_state.more \<omega>2 \<Longrightarrow>
+     \<omega>1 \<le> \<omega>2"
+  unfolding less_eq_full_total_state_ext_def
+  by auto
 
 lemma less_eq_full_total_stateD:
   assumes "\<omega>1 \<le> \<omega>2"
   shows "get_store_total \<omega>1 = get_store_total \<omega>2 \<and>
-         get_trace_total \<omega>1 = get_trace_total \<omega>2 \<and>         
+         dom (get_trace_total \<omega>1) = dom (get_trace_total \<omega>2) \<and>      
+         (\<forall>lbl \<phi> \<phi>'. (get_trace_total \<omega>1 lbl = Some \<phi> \<and> 
+                      get_trace_total \<omega>2 lbl = Some \<phi>') \<longrightarrow> \<phi> \<le> \<phi>') \<and>   
          get_total_full \<omega>1 \<le> get_total_full \<omega>2 \<and>
          full_total_state.more \<omega>1 = full_total_state.more \<omega>2"
   using assms
   unfolding less_eq_full_total_state_ext_def
-  by blast
+  by argo
 
 lemma less_eq_full_total_stateE:
   assumes "\<omega>1 \<le> \<omega>2" and
           "get_store_total \<omega>1 = get_store_total \<omega>2 \<Longrightarrow>
-           get_trace_total \<omega>1 = get_trace_total \<omega>2 \<Longrightarrow>
+           dom (get_trace_total \<omega>1) = dom (get_trace_total \<omega>2) \<Longrightarrow>   
+           (\<forall>lbl \<phi> \<phi>'. (get_trace_total \<omega>1 lbl = Some \<phi> \<and> 
+                        get_trace_total \<omega>2 lbl = Some \<phi>') \<longrightarrow> \<phi> \<le> \<phi>') \<Longrightarrow>
            get_total_full \<omega>1 \<le> get_total_full \<omega>2 \<Longrightarrow>
            full_total_state.more \<omega>1 = full_total_state.more \<omega>2 \<Longrightarrow> P"
   shows P
@@ -286,7 +343,7 @@ proof -
   thus ?thesis
     using assms
     unfolding less_eq_full_total_state_ext_def
-    by simp
+    by auto
 qed
 
 definition empty_full_total_state :: "'a store \<Rightarrow> 'a total_trace \<Rightarrow> 'a total_heap \<Rightarrow> 'a predicate_heap \<Rightarrow> 'a full_total_state"
